Split shared things into Utils, some progress on decidability lemma for termination

Mixed.v
@@ -2,42 +2,42 @@ From Coq Require Import
      List
      Lia
      Relations
-     Arith.Arith.
+     Arith.Arith
+     Program.Equality.
 
 From ExtLib Require Import
      Structures.Maps
+     Structures.Monoid
      Data.Map.FMapAList
      Core.RelDec
      Data.Nat
      Structures.Monad
      Structures.MonadLaws.
 
+From RDS Require Import Utils.
+
 Import ListNotations.
 
 Set Implicit Arguments.
+Set Asymmetric Patterns.
+Set Printing Projections.
 
 Module Mixed.
-  Variable uid : Set.
-  Variable var : Set.
-
-  Parameter eqdec_var: RelDec (@eq var).
-  Parameter eqdec_uid: RelDec (@eq uid).
-
-  Global Existing Instance eqdec_var.
-  Global Existing Instance eqdec_uid.
+  Include Utils.
 
   Inductive loop_outcome(acc: Type) :=
   | Done (a : acc)
   | Again (a : acc).
 
   (** cmd *)
-  Inductive cmd : Type -> Type :=
+  Inductive cmd : Set -> Type :=
   | Return {A: Set} (r : A) : cmd A
   | Bind {A B} (c1 : cmd A)
          (c2 : A -> cmd B): cmd B
-  | Recv (a : var)(from: uid): cmd var
+  | Recv {A: Set}(a : var)(from: uid): cmd A
   | Send {A: Set} (payload: A) (to: uid) : cmd unit
   | Store {A: Set}(reg: var)(value: A): cmd unit
+  | Restart: cmd unit
   | Load {A: Set} (reg: var): cmd A
   | Loop {acc : Set} (init : acc)
          (body : acc -> cmd (loop_outcome acc)) : cmd acc.
@@ -46,17 +46,11 @@ Module Mixed.
   Notation "'for' x := i 'loop' c1 'done'" :=
     (Loop i (fun x => c1)) (right associativity, at level 80).
 
-  (** Heap is map *)
-  Record dyn := {
-      type: Type;
-      value: type
-    }.
-  
-  (** No state for now, except my own uid *)
-  Definition local := (uid * alist var dyn)%type.
-                
+  (* Agent has state and a program *)
+  Notation agent T := (local * cmd T)%type.
+
   (** LTS *)
-  Inductive lstep : forall A, local * cmd A -> local * cmd A -> Prop :=
+  Inductive lstep : forall A, agent A -> agent A -> Prop :=
   | StepBindRecur : forall result result' l l'
                       (c1 c1' : cmd result')
                       (c2 : result' -> cmd result),
@@ -73,21 +67,117 @@ Module Mixed.
                                                    | Again a => Loop a body
                                                     end)
   | StepStore: forall (A: Set) reg u ctx (val: A),
-      lstep ((u, ctx), @Store A reg val)
-            ((u, add reg {| type:= A; value:=val |} ctx),
+      lstep (u, ctx, @Store A reg val)
+            (u, add reg {| type:= A; value:=val |} ctx,
               Return tt)
-  | StepLoad: forall (A: Set) reg u (val: A) ctx,
+  | StepLoadFound: forall (A: Set) reg u (val: A) ctx,
       lookup reg ctx = Some {| type := A; value := val |} -> 
-      lstep ((u, ctx), Load reg)
-            ((u, ctx), Return val).
-  
+      lstep (u, ctx, Load reg)
+            (u, ctx, Return val)
+  | StepLoadError: forall (A: Set) reg u (val: A) ctx,
+      lookup reg ctx = None ->
+      lstep (u, ctx, Load reg)
+            (u, ctx, Restart).
+
+  Notation "a '-[' n ']->' b" := (@trsys_nat (agent _) (@lstep _) n a b) (at level 65, right associativity).
 
   Inductive blocked: forall A, cmd A -> Prop :=
-  | RecvBlock: forall a u, blocked (Recv a u)
-  | SendBlock: forall {A: Set} {a: A} u, blocked (Send a u).
+  | RecvBlock: forall {A: Set} a u, blocked (@Recv A a u)
+  | SendBlock: forall {A: Set} {a: A} u, blocked (Send a u)
+  | RestartBlock: blocked (Restart)
+  | BindBlock: forall A B (p: cmd A)(c: A -> cmd B), blocked p -> blocked (x <- p; c x).
 
   Inductive returned: forall A, cmd A -> Prop :=
   | DoneCmd: forall {A: Set} {n: A}, returned (Return n).
 
+  Hint Constructors blocked returned lstep trsys_nat: core.
 
+  Lemma agent_lstep_terminates_or_blocked:
+    forall A ctx p,
+      blocked p \/ returned p \/ (exists ctx' p', @lstep A (ctx, p) (ctx', p')).
+  Proof with eauto.
+    intros.
+    induction p.
+    - right; left... 
+    - destruct IHp.
+      + left... 
+      + destruct H0.
+        * dependent destruction H0.
+          right. right.
+          exists ctx. exists (c2 n)...
+        * destruct H0 as [ctx' [p' H']].
+          right. right.
+          exists ctx'.
+          exists (x <- p'; c2 x)...
+    - left...
+    - left...
+    - right. right. destruct ctx.
+      exists (u, add reg {| type := A; value := value0 |} a).
+      exists (Return tt)...
+    - left...
+    - right. right. exists ctx.
+      destruct ctx.
+      destruct (lookup reg a) eqn:Hload.
+      + dependent destruction d.
+        exists (Return value0).
+      (* Load could fail add exceptions! *)
+  Admitted.
+
+  Lemma agent_terminates_or_blocked:
+    forall (a: agent nat), exists ctx' p' n,
+      (a -[n]-> (ctx', p')) /\ (blocked p' \/ returned p').
+  Proof with eauto.
+    intros [[uid heap] prog].
+    induction prog.
+    - (* Return *)
+      exists (uid, heap); exists (Return r); exists 0...
+    - (* Bind: inductive case *)
+      destruct IHprog as [ctx' [p' [n' [H1 [H2|H2]]]]].
+      dependent induction H1.
+      + exists (uid, heap).
+        exists (x <- p'; c2 x).
+        eexists. 
+        split.
+        * eapply refl.
+        * left. econstructor.
+          apply H2.
+      + destruct b; subst.
+
+        specialize (IHtrsys_nat uid heap _ prog c2 H l _ eq_refl
+                                JMeq_refl
+                                JMeq_refl
+                                JMeq_refl
+                   ).
+        
+        exists (ctx').
+        exists (x <- c; c2 x).
+        eexists.
+        split.
+        * e
+          eapply refl.
+          eapply StepBindRecur.
+          eapply trans.
+          inversion H1; subst.
+          -- inversion H1; subst.
+          eapply StepBindRecur.
+          econstructor.
+          
+      destruct 
+      eexists.
+      eexists.
+      eexists.
+      split.
+      + eapply econstructor.
+      + 
+      admit.
+    - (* Recv *)
+      exists (uid, heap); exists (Recv a from0); exists 0...
+    - (* Send *)
+      exists (uid, heap); exists (Send payload0 to0); exists 0...
+    - (* Store *)
+      exists (uid, (add reg {| type := A; value := value0 |} heap)).
+      eexists. exists 1...
+    - (* Load *)
+  Admitted.
+  
 End Mixed.
