Utils.v
@@ -1,0 +1,61 @@
+From Coq Require Import
+     Relations
+     List.
+
+From ExtLib Require Import
+     Core.RelDec
+     Data.Nat
+     Structures.Maps
+     Structures.Monoid
+     Data.Map.FMapAList.
+
+Import ListNotations.
+Set Implicit Arguments.
+
+Module Utils.
+  Variable uid : Set.
+  Variable var : Set.
+
+  Parameter eqdec_var: RelDec (@eq var).
+  Parameter eqdec_uid: RelDec (@eq uid).
+
+  Global Existing Instance eqdec_var.
+  Global Existing Instance eqdec_uid.
+
+  Record dyn := {
+      type: Set;
+      value: type
+    }.
+
+  Record message := {
+      from: uid;
+      to: uid;
+      payload: dyn
+    }.
+
+  Inductive label :=
+  | Msg (m : message)
+  | Read (user: uid)(v: var)
+  | Write (user: uid)(v: var)(val: dyn)
+  | Silent.
+
+  (** Backwards *)
+  Inductive trsys_nat A (R: A -> A -> Prop): nat -> relation A :=
+  | refl: forall a, trsys_nat R 0 a a
+  | trans: forall a b c n, 
+      trsys_nat R n a b ->
+      R b c ->
+      trsys_nat R (S n) a c.
+
+  (** State := my own uid and a valuation context (heap) *)
+  Notation local := (uid * alist var dyn)%type (only parsing).
+
+  Inductive trsys_label A (R: A -> label -> A -> Prop): list label -> relation A :=
+  | reflL: forall a, trsys_label R [] a a
+  | transL: forall a b c h tr, R a h b ->
+                         trsys_label R tr b c ->
+                         trsys_label R (h :: tr) a c.
+
+  Hint Constructors trsys_label: core.
+
+End Utils.
